src/sequential/SeqLiftSim.v
@@ -38,11 +38,15 @@ Require Import Lia.
 Require Import JoinedView.
 Require Import SeqLift.
 Require Import SeqLiftStep.
-Require Import gSimulation.
+Require Import SeqLiftCertification.
+Require Import DelayedSimulation.
 Require Import Simple.
 
 Require Import Pred.
 
+Require Import SimAux.
+Require Import FlagAux.
+Require Import SeqAux.
 
 Variant initial_finalized: Messages.t :=
   | initial_finalized_intro
@@ -83,74 +87,1545 @@ Definition initial_vers: versions :=
   fun loc ts =>
     if (Time.eq_dec ts Time.bot) then Some (fun _ => 0) else None.
 
+Require Import Program.
+
+Module CertOracle.
+  Definition t := Loc.t -> Const.t.
+
+  Definition output (e: ProgramEvent.t): Oracle.output :=
+    Oracle.mk_output
+      (if is_accessing e then Some Perm.high else None)
+      (if is_acquire e then Some (fun _ => Perm.low, fun _ => Const.undef) else None)
+      (if is_release e then Some (fun _ => Perm.high) else None)
+  .
+
+  Variant step (e: ProgramEvent.t) (i: Oracle.input) (o: Oracle.output) (vs: t): t -> Prop :=
+    | step_read
+        loc ord
+        (EVENT: e = ProgramEvent.read loc (vs loc) ord)
+        (INPUT: Oracle.wf_input e i)
+        (OUTPUT: o = output e)
+      :
+      step e i o vs vs
+    | step_write
+        loc val ord
+        (EVENT: e = ProgramEvent.write loc val ord)
+        (INPUT: Oracle.wf_input e i)
+        (OUTPUT: o = output e)
+      :
+      step e i o vs (fun loc0 => if Loc.eq_dec loc0 loc then val else vs loc0)
+    | step_update
+        loc valw ordr ordw
+        (EVENT: e = ProgramEvent.update loc (vs loc) valw ordr ordw)
+        (INPUT: Oracle.wf_input e i)
+        (OUTPUT: o = output e)
+      :
+      step e i o vs (fun loc0 => if Loc.eq_dec loc0 loc then valw else vs loc0)
+    | step_fence
+        ordr ordw
+        (EVENT: e = ProgramEvent.fence ordr ordw)
+        (INPUT: Oracle.wf_input e i)
+        (OUTPUT: o = output e)
+      :
+      step e i o vs vs
+    | step_syscall
+        ev
+        (EVENT: e = ProgramEvent.syscall ev)
+        (INPUT: Oracle.wf_input e i)
+        (OUTPUT: o = output e)
+      :
+      step e i o vs vs
+  .
+
+  Definition to_oracle (vs: t): Oracle.t := @Oracle.mk t step vs.
+
+  Lemma to_oracle_wf vs: Oracle.wf (to_oracle vs).
+  Proof.
+    revert vs. pcofix CIH. i. pfold. econs.
+    { i. dependent destruction STEP. inv STEP.
+      { splits; auto. red. splits; ss; des_ifs. }
+      { splits; auto. red. splits; ss; des_ifs. }
+      { splits; auto. red. splits; ss; des_ifs. }
+      { splits; auto. red. splits; ss; des_ifs. }
+      { splits; auto. red. splits; ss; des_ifs. }
+    }
+    { i. exists (vs loc). splits.
+      { econs. esplits.
+        { econs. eapply step_read; eauto. }
+        { red. splits; ss; des_ifs. }
+      }
+      { i. econs. esplits.
+        { econs. eapply step_update; eauto. }
+        { red. splits; ss; des_ifs. }
+      }
+    }
+    { i. econs. esplits.
+      { econs. eapply step_write; eauto. }
+      { red. splits; ss; des_ifs. }
+    }
+    { i. econs. esplits.
+      { econs. eapply step_fence; eauto. }
+      { red. splits; ss; des_ifs. }
+    }
+    { i. econs. esplits.
+      { econs. eapply step_syscall; eauto. }
+      { red. splits; ss; des_ifs. }
+    }
+  Qed.
+End CertOracle.
+
+
 Section LIFT.
-  Let world := (Mapping.ts * versions)%type.
+  Variable loc_na: Loc.t -> Prop.
+  Variable loc_at: Loc.t -> Prop.
+  Hypothesis LOCDISJOINT: forall loc (NA: loc_na loc) (AT: loc_at loc), False.
 
-  Let world_bot: world := (fun _ => initial_mapping, initial_vers).
+  Definition _nomix
+             (nomix: forall (lang: language) (st: lang.(Language.state)), Prop)
+             (lang: language) (st: lang.(Language.state)): Prop :=
+    forall st1 e
+           (STEP: lang.(Language.step) e st st1),
+      (<<NA: forall l c (NA: is_atomic_event e = false) (ACC: is_accessing e = Some (l, c)), loc_na l>>) /\
+        (<<AT: forall l c (AT: is_atomic_event e = true) (ACC: is_accessing e = Some (l, c)), loc_at l>>) /\
+        (<<CONT: nomix lang st1>>)
+  .
 
-  Let world_messages_le (msgs: Messages.t) (w0: world) (w1: world): Prop :=
-        let (f0, vers0) := w0 in
-        let (f1, vers1) := w1 in
-        Mapping.les f0 f1 /\ versions_le vers0 vers1.
+  Definition nomix := paco2 _nomix bot2.
+  Arguments nomix: clear implicits.
 
-  Let sim_memory (b: bool) (w: world) (views: Loc.t -> Time.t -> list View.t)
-      (mem_src: Memory.t) (mem_tgt: Memory.t): Prop :=
-        let (f, vers) := w in
-        sim_memory (fun _ => None) f vers mem_src mem_tgt.
-
-  Let sim_timemap (w: world)
-      (tm_src: TimeMap.t) (tm_tgt: TimeMap.t): Prop :=
-        let (f, vers) := w in
-        sim_timemap (fun _ => True) f (Mapping.vers f) tm_src tm_tgt.
-
-  Let sim_local (w: world) (views: Loc.t -> Time.t -> list View.t) (lc_src: Local.t) (lc_tgt: Local.t): Prop :=
-        let (f, vers) := w in
-        sim_local f vers (fun _ => None) (fun _ => None) lc_src lc_tgt.
-
-
-
-  Lemma world_messages_le_PreOrder: forall msgs, PreOrder (world_messages_le msgs).
+  Lemma nomix_mon: monotone2 _nomix.
   Proof.
-    ii. econs.
-    { ii. red. des_ifs. splits; auto.
-      { refl. }
-      { refl. }
-    }
-    { ii. unfold world_messages_le in *. des_ifs. des. splits; auto.
-      { etrans; eauto. }
-      { etrans; eauto. }
-    }
+    ii. exploit IN; eauto. i. des. splits.
+    { i. hexploit NA; eauto. }
+    { i. hexploit AT; eauto. }
+    { auto. }
+  Qed.
+  #[local] Hint Resolve nomix_mon: paco.
+
+
+  Definition sim_seq_interference lang_src lang_tgt sim_terminal p0 D st_src st_tgt :=
+    forall p1 (PERM: Perms.le p1 p0),
+      @sim_seq lang_src lang_tgt sim_terminal p1 D st_src st_tgt.
+
+  Lemma sim_seq_interference_mon lang_src lang_tgt sim_terminal p0 D st_src st_tgt
+        (SIM: @sim_seq_interference _ _ sim_terminal p0 D st_src st_tgt)
+        p1 (PERM: Perms.le p1 p0)
+    :
+    @sim_seq_interference lang_src lang_tgt sim_terminal p1 D st_src st_tgt.
+  Proof.
+    ii. eapply SIM. etrans; eauto.
   Qed.
 
-  Lemma sim_local_memory_bot:
-    forall w views lc_src lc_tgt
-           (SIM: sim_local w views lc_src lc_tgt)
-           (BOT: (Local.promises lc_tgt) = Memory.bot),
-      (Local.promises lc_src) = Memory.bot.
+  Lemma sim_seq_interference_sim_seq lang_src lang_tgt sim_terminal p D st_src st_tgt
+        (SIM: @sim_seq_interference _ _ sim_terminal p D st_src st_tgt)
+    :
+    @sim_seq lang_src lang_tgt sim_terminal p D st_src st_tgt.
   Proof.
-    ii. unfold sim_local in *. des_ifs. inv SIM. ss. subst.
-    inv PROMISES. eapply Memory.ext. ii.
-    rewrite Memory.bot_get.
-    destruct (Memory.get loc ts prom_src) eqn:EQ; auto. destruct p.
-    hexploit SOUND; eauto. i. des; ss. rewrite Memory.bot_get in GET. ss.
+    eapply SIM. refl.
   Qed.
+
+  Lemma sim_seq_release lang_src lang_tgt sim_terminal
+        p0 d0 st_src0 st_tgt0
+        (SIM: sim_seq_at_step_case (@sim_seq lang_src lang_tgt sim_terminal) p0 d0 st_src0 st_tgt0)
+    :
+    forall st_tgt1 e_tgt
+           (STEP_TGT: lang_tgt.(Language.step) e_tgt st_tgt0.(SeqState.state) st_tgt1)
+           (ATOMIC: is_atomic_event e_tgt)
+           (RELEASE: is_release e_tgt),
+    exists st_src1 st_src2 e_src,
+      (<<STEPS: rtc (SeqState.na_step p0 MachineEvent.silent) st_src0 st_src1>>) /\
+        (<<STEP: lang_src.(Language.step) e_src st_src1.(SeqState.state) st_src2>>) /\
+        (<<EVENT: ProgramEvent.le e_tgt e_src>>) /\
+        (<<SIM: forall i_tgt o p1 mem_tgt
+                       (INPUT: SeqEvent.wf_input e_tgt i_tgt)
+                       (OUTPUT: Oracle.wf_output e_tgt o)
+                       (STEP_TGT: SeqEvent.step i_tgt o p0 st_tgt0.(SeqState.memory) p1 mem_tgt),
+          exists i_src mem_src d1,
+            (<<STEP_SRC: SeqEvent.step i_src o p0 st_src1.(SeqState.memory) p1 mem_src>>) /\
+              (<<MATCH: SeqEvent.input_match d0 d1 i_src i_tgt>>) /\
+              (<<INPUT: SeqEvent.wf_input e_src i_src>>) /\
+              (<<SIM: sim_seq_interference
+                        _ _ sim_terminal
+                        p1 d1
+                        (SeqState.mk _ st_src2 mem_src)
+                        (SeqState.mk _ st_tgt1 mem_tgt)>>)>>).
+  Proof.
+    i. exploit SIM; eauto. i. des. esplits; eauto.
+    i. hexploit SIM0; eauto. i. des. esplits; eauto.
+    inv STEP_TGT0. inv REL.
+    { red in OUTPUT. des. hexploit RELEASE1; eauto.
+      i. rewrite <- H in *. ss.
+    }
+    ii.
+    hexploit (SIM0 i_tgt (Oracle.mk_output o.(Oracle.out_access) o.(Oracle.out_acquire) (Some p1))); eauto.
+    { red in OUTPUT. des. red. splits; auto. }
+    { econs.
+      { eauto. }
+      { eauto. }
+      { ss. rewrite <- H0. econs 2; eauto. }
+    }
+  Admitted.
+
+  Definition world := (Mapping.ts * versions * Memory.t)%type.
+
+  Definition world_bot: world := (fun _ => initial_mapping, initial_vers, Memory.init).
+
+  Definition world_messages_le (msgs_src msgs_tgt: Messages.t) (w0: world) (w1: world): Prop :=
+        match w0, w1 with
+        | (f0, vers0, mem_src0), (f1, vers1, mem_src1) =>
+            forall (WF: Mapping.wfs f0),
+              (<<MAPLE: Mapping.les f0 f1>>) /\ (<<VERLE: versions_le vers0 vers1>>) /\
+                (<<MEMSRC: Memory.future_weak mem_src0 mem_src1>>) /\
+                (<<FUTURE: map_future_memory f0 f1 mem_src1>>) /\
+                (<<WF: Mapping.wfs f1>>)
+        end
+  .
+
+  Program Instance world_messages_le_PreOrder msgs_src msgs_tgt: PreOrder (world_messages_le msgs_src msgs_tgt).
+  Next Obligation.
+    unfold world_messages_le. ii. des_ifs. splits.
+    { refl. }
+    { refl. }
+    { refl. }
+    { eapply map_future_memory_refl. }
+    { auto. }
+  Qed.
+  Next Obligation.
+    unfold world_messages_le. ii. des_ifs. i.
+    hexploit H; eauto. i. des.
+    hexploit H0; eauto. i. des.
+    splits.
+    { etrans; eauto. }
+    { etrans; eauto. }
+    { etrans; eauto. }
+    { eapply map_future_memory_trans; eauto. }
+    { eauto. }
+  Qed.
+
+  Local Existing Instances world_messages_le_PreOrder.
 
   Lemma world_messages_le_mon:
-    forall msgs0 msgs1 w0 w1
-           (LE: world_messages_le msgs1 w0 w1)
-           (MSGS: msgs0 <4= msgs1),
-      world_messages_le msgs0 w0 w1.
+    forall msgs_src0 msgs_tgt0 msgs_src1 msgs_tgt1 w0 w1
+           (LE: world_messages_le msgs_src1 msgs_tgt1 w0 w1)
+           (MSGSRC: msgs_src0 <4= msgs_src1)
+           (MSGTGT: msgs_tgt0 <4= msgs_tgt1),
+      world_messages_le msgs_src0 msgs_tgt0 w0 w1.
   Proof.
-    unfold world_messages_le. ii. des_ifs.
+    unfold world_messages_le. i. des_ifs.
   Qed.
+
+  Definition sim_memory_lift: forall (w: world) (mem_src mem_tgt:Memory.t), Prop :=
+    fun w mem_src mem_tgt =>
+      match w with
+      | (f, vers, mem_src') =>
+          (<<MEMSRC: mem_src = mem_src'>>) /\
+            (<<SIM: sim_memory (fun _ => None) f vers mem_src mem_tgt>>)
+      end.
+
+  Definition sim_timemap_lift: forall (w: world) (tm_src: TimeMap.t) (tm_tgt: TimeMap.t), Prop :=
+    fun w tm_src tm_tgt =>
+      match w with
+      | (f, vers, _) =>
+          (<<SIM: sim_timemap (fun _ => True) f (Mapping.vers f) tm_src tm_tgt>>)
+      end.
+
+  Variant sim_val_lift: forall
+      (p: Perm.t)
+      (sv_src: Const.t) (sv_tgt: Const.t)
+      (v_src: option Const.t) (v_tgt: option Const.t), Prop :=
+    | sim_val_lift_low
+        sv_src sv_tgt
+      :
+      sim_val_lift Perm.low sv_src sv_tgt None None
+    | sim_val_lift_high
+        sv_src sv_tgt v_src v_tgt
+        (VALSRC: Const.le sv_src v_src)
+        (VALTGT: Const.le v_tgt sv_tgt)
+      :
+      sim_val_lift Perm.high sv_src sv_tgt (Some v_src) (Some v_tgt)
+  .
+
+  Definition sim_vals_lift
+             (p: Perms.t) (svs_src: ValueMap.t) (svs_tgt: ValueMap.t)
+             (vs_src: Loc.t -> option Const.t) (vs_tgt: Loc.t -> option Const.t): Prop :=
+    forall loc (NA: loc_na loc), sim_val_lift (p loc) (svs_src loc) (svs_tgt loc) (vs_src loc) (vs_tgt loc).
+
+  Variant sim_flag_lift
+          (d: Flag.t) (sflag_src: Flag.t) (sflag_tgt: Flag.t)
+          (flag_src: option Time.t) (flag_tgt: option Time.t): Prop :=
+    | sim_flag_lift_intro
+        (TGT: flag_tgt -> Flag.join flag_src (Flag.join d sflag_tgt))
+        (SRC: sflag_src = flag_src)
+  .
+
+  Definition sim_flags_lift
+             (d: Flags.t) (sflag_src: Flags.t) (sflag_tgt: Flags.t)
+             (flag_src: Loc.t -> option Time.t) (flag_tgt: Loc.t -> option Time.t): Prop :=
+    forall loc (NA: loc_na loc), sim_flag_lift (d loc) (sflag_src loc) (sflag_tgt loc) (flag_src loc) (flag_tgt loc).
+
+  Variant sim_state_lift:
+    forall (w: world)
+           (smem_src: SeqMemory.t) (smem_tgt: SeqMemory.t)
+           (p: Perms.t)
+           (D: Flags.t)
+           (mem_src: Memory.t)
+           (mem_tgt: Memory.t)
+           (lc_src: Local.t)
+           (lc_tgt: Local.t)
+           (sc_src: TimeMap.t)
+           (sc_tgt: TimeMap.t), Prop :=
+    | sim_state_lift_intro
+        svs_src sflag_src svs_tgt sflag_tgt
+        p D f vers flag_src flag_tgt vs_src vs_tgt
+        mem_src mem_tgt lc_src lc_tgt sc_src sc_tgt
+        (SIM: SeqLiftStep.sim_thread f vers flag_src flag_tgt vs_src vs_tgt mem_src mem_tgt lc_src lc_tgt sc_src sc_tgt)
+        (VALS: sim_vals_lift p svs_src svs_tgt vs_src vs_tgt)
+        (FLAGS: sim_flags_lift D sflag_src sflag_tgt flag_src flag_tgt)
+        (WF: Mapping.wfs f)
+        (VERS: versions_wf f vers)
+        (VERSIONED: versioned_memory vers mem_tgt)
+        (ATLOCS: forall loc (AT: loc_at loc),
+            (<<FLAGSRC: flag_src loc = None>>) /\
+              (<<FLAGTGT: flag_tgt loc = None>>) /\
+              (<<VAL: option_rel Const.le (vs_tgt loc) (vs_src loc)>>))
+      :
+      sim_state_lift
+        (f, vers, mem_tgt)
+        (SeqMemory.mk svs_src sflag_src) (SeqMemory.mk svs_tgt sflag_tgt)
+        p D
+        mem_src mem_tgt lc_src lc_tgt sc_src sc_tgt
+  .
+
+  Lemma rtc_steps_thread_failure lang th0 th1
+        (STEPS: rtc (@Thread.tau_step lang) th0 th1)
+        (FAILURE: Thread.steps_failure th1)
+    :
+    Thread.steps_failure th0.
+  Proof.
+    unfold Thread.steps_failure in *. des. esplits.
+    { etrans; eauto. }
+    { eauto. }
+    { eauto. }
+  Qed.
+
+  Lemma sim_lift_tgt_na_write_step:
+    forall
+      w p D smem_src smem_tgt0 mem_src0 mem_tgt0 lc_src0 lc_tgt0 sc_src0 sc_tgt0
+      mem_tgt1 lc_tgt1 sc_tgt1
+      loc from to val msgs kinds kind
+      (LIFT: sim_state_lift w smem_src smem_tgt0 p D mem_src0 mem_tgt0 lc_src0 lc_tgt0 sc_src0 sc_tgt0)
+      (STEP: Local.write_na_step lc_tgt0 sc_tgt0 mem_tgt0 loc from to val Ordering.na lc_tgt1 sc_tgt1 mem_tgt1 msgs kinds kind)
+      (NALOCS: loc_na loc)
+      (LOWER: mem_tgt1 = mem_tgt0)
+      (CONSISTENT: Local.promise_consistent lc_tgt1)
+      (WF_SRC: Local.wf lc_src0 mem_src0)
+      (WF_TGT: Local.wf lc_tgt0 mem_tgt0)
+      (SC_SRC: Memory.closed_timemap sc_src0 mem_src0)
+      (SC_TGT: Memory.closed_timemap sc_tgt0 mem_tgt0)
+      (MEM_SRC: Memory.closed mem_src0)
+      (MEM_TGT: Memory.closed mem_tgt0)
+      lang_src st_src,
+    exists lc_src1 mem_src1 sc_src1 me smem_tgt1,
+      (<<STEPS: rtc (@Thread.tau_step lang_src) (Thread.mk _ st_src lc_src0 sc_src0 mem_src0) (Thread.mk _ st_src lc_src1 sc_src1 mem_src1)>>) /\
+        (<<STEP: SeqState.na_local_step p me (ProgramEvent.write loc val Ordering.na) smem_tgt0 smem_tgt1>>) /\
+        (<<LIFT: forall (NORMAL: me <> MachineEvent.failure),
+            sim_state_lift w smem_src smem_tgt1 p D mem_src1 mem_tgt1 lc_src1 lc_tgt1 sc_src1 sc_tgt1>>)
+  .
+  Proof.
+    i. inv LIFT. destruct (vs_tgt loc) eqn:VAL.
+    { hexploit sim_thread_tgt_write_na; eauto. i. des. esplits.
+      { eauto. }
+      { econs 3; eauto. }
+      { i. subst. econs; eauto.
+        { ii. unfold ValueMap.write. des_ifs; ss.
+          { des_ifs. hexploit (VALS loc); auto. i.
+            rewrite VAL in *. rewrite Heq0 in *.
+            inv H. econs; eauto. refl.
+          }
+          { eapply VALS; eauto. }
+        }
+        { ss. unfold Flags.update. ii. des_ifs.
+          { econs; ss; auto.
+            { i. destruct (flag_src loc), (D loc); ss. }
+            { eapply FLAGS; auto. }
+          }
+          { eapply FLAGS; auto. }
+        }
+        { i. ss. des_ifs.
+          { exfalso. eapply LOCDISJOINT; eauto. }
+          { eapply ATLOCS; eauto. }
+        }
+      }
+    }
+    { esplits.
+      { refl. }
+      { econs 3; eauto.}
+      { i. hexploit (VALS loc); auto. i.
+        rewrite VAL in H. inv H.
+        rewrite <- H1 in *. ss.
+      }
+    }
+  Qed.
+
+  Lemma sim_lift_tgt_na_local_step:
+    forall
+      w p D smem_src smem_tgt0 mem_src0 mem_tgt0 lc_src0 lc_tgt0 sc_src0 sc_tgt0
+      e pe mem_tgt1 lc_tgt1 sc_tgt1
+      (LIFT: sim_state_lift w smem_src smem_tgt0 p D mem_src0 mem_tgt0 lc_src0 lc_tgt0 sc_src0 sc_tgt0)
+      (STEP: Local.program_step e lc_tgt0 sc_tgt0 mem_tgt0 lc_tgt1 sc_tgt1 mem_tgt1)
+      (EVENT: ThreadEvent.get_program_event e = pe)
+      (NA: ~ is_atomic_event pe)
+      (NALOCS: forall loc val (ACCESS: is_accessing pe = Some (loc, val)), loc_na loc)
+      (LOWER: is_na_write e -> mem_tgt1 = mem_tgt0)
+
+      (CONSISTENT: Local.promise_consistent lc_tgt1)
+      (WF_SRC: Local.wf lc_src0 mem_src0)
+      (WF_TGT: Local.wf lc_tgt0 mem_tgt0)
+      (SC_SRC: Memory.closed_timemap sc_src0 mem_src0)
+      (SC_TGT: Memory.closed_timemap sc_tgt0 mem_tgt0)
+      (MEM_SRC: Memory.closed mem_src0)
+      (MEM_TGT: Memory.closed mem_tgt0)
+      lang_src st_src,
+    exists lc_src1 mem_src1 sc_src1 me smem_tgt1,
+      (<<STEPS: rtc (@Thread.tau_step lang_src) (Thread.mk _ st_src lc_src0 sc_src0 mem_src0) (Thread.mk _ st_src lc_src1 sc_src1 mem_src1)>>) /\
+      (<<STEP: SeqState.na_local_step p me pe smem_tgt0 smem_tgt1>>) /\
+        (<<LIFT: forall (NORMAL: me <> MachineEvent.failure),
+            sim_state_lift w smem_src smem_tgt1 p D mem_src1 mem_tgt1 lc_src1 lc_tgt1 sc_src1 sc_tgt1>>)
+  .
+  Proof.
+    i. inv STEP; ss.
+    { esplits.
+      { refl. }
+      { econs 1. }
+      { eauto. }
+    }
+    { inv LIFT. destruct ord; ss. hexploit sim_thread_tgt_read_na; eauto.
+      i. des. esplits.
+      { refl. }
+      { econs 2; eauto. i. ss. hexploit (VALS loc); eauto. i. inv H0.
+        { des_ifs. }
+        hexploit VAL; eauto. i. etrans; eauto.
+      }
+      { i. econs; eauto. }
+    }
+    { destruct ord; ss. eapply local_write_step_write_na_step in LOCAL.
+      eapply sim_lift_tgt_na_write_step; eauto.
+    }
+    { esplits.
+      { refl. }
+      { econs 5. red. destruct ordr, ordw; ss; auto. }
+      { ss. }
+    }
+    { esplits.
+      { refl. }
+      { econs 4. }
+      { ss. }
+    }
+    { destruct ord; ss. eapply sim_lift_tgt_na_write_step; eauto. }
+    { inv LIFT. destruct ord; ss. hexploit sim_thread_tgt_read_na_racy; eauto.
+      i. esplits.
+      { refl. }
+      { econs 2; eauto. i. hexploit (VALS loc); eauto. i.
+        rewrite H in H1. inv H1.
+        rewrite <- H3 in *. ss.
+      }
+      { i. econs; eauto. }
+    }
+    { inv LIFT. destruct ord; ss. hexploit sim_thread_tgt_write_na_racy; eauto.
+      i. esplits.
+      { refl. }
+      { econs 3; eauto. }
+      { i. hexploit (VALS loc); eauto. i. rewrite H in H0. inv H0.
+        rewrite <- H2 in *. ss.
+      }
+    }
+    { esplits.
+      { refl. }
+      { econs 5. red. destruct ordr, ordw; ss; auto. }
+      { ss. }
+    }
+  Qed.
+
+  Lemma sim_lift_src_na_local_step:
+    forall
+      w p D smem_src0 smem_tgt mem_src0 mem_tgt lc_src0 lc_tgt sc_src0 sc_tgt
+      pe me smem_src1
+      (LIFT: sim_state_lift w smem_src0 smem_tgt p D mem_src0 mem_tgt lc_src0 lc_tgt sc_src0 sc_tgt)
+      (STEP: SeqState.na_local_step p me pe smem_src0 smem_src1)
+      (NA: ~ is_atomic_event pe)
+      (NALOCS: forall loc val (ACCESS: is_accessing pe = Some (loc, val)), loc_na loc)
+
+      (CONSISTENT: Local.promise_consistent lc_tgt)
+      (WF_SRC: Local.wf lc_src0 mem_src0)
+      (WF_TGT: Local.wf lc_tgt mem_tgt)
+      (SC_SRC: Memory.closed_timemap sc_src0 mem_src0)
+      (SC_TGT: Memory.closed_timemap sc_tgt mem_tgt)
+      (MEM_SRC: Memory.closed mem_src0)
+      (MEM_TGT: Memory.closed mem_tgt)
+      lang_src st_src,
+    exists lc_src1 mem_src1 sc_src1 lc_src2 mem_src2 sc_src2 e,
+      (<<STEPS: rtc (@Thread.tau_step lang_src) (Thread.mk _ st_src lc_src0 sc_src0 mem_src0) (Thread.mk _ st_src lc_src1 sc_src1 mem_src1)>>) /\
+        (<<STEP: Local.program_step e lc_src1 sc_src1 mem_src1 lc_src2 sc_src2 mem_src2>>) /\
+        (<<MACHINE: ThreadEvent.get_machine_event e = me>>) /\
+        (<<EVENT: ThreadEvent.get_program_event e = pe>>) /\
+        (<<LIFT: forall (NORMAL: ThreadEvent.get_machine_event e <> MachineEvent.failure),
+            sim_state_lift w smem_src1 smem_tgt p D mem_src2 mem_tgt lc_src2 lc_tgt sc_src2 sc_tgt>>)
+  .
+  Proof.
+    i. inv STEP.
+    { esplits.
+      { refl. }
+      { eapply Local.step_silent. }
+      { ss. }
+      { ss. }
+      { auto. }
+    }
+    { inv LIFT. ss. hexploit (VALS loc); eauto. i. inv H.
+      { hexploit sim_thread_src_read_na_racy; eauto. i.
+        esplits.
+        { refl. }
+        { eapply Local.step_racy_read; eauto. }
+        { ss. }
+        { ss. destruct ord; ss. }
+        { i. econs; eauto. }
+      }
+      { hexploit sim_thread_src_read_na.
+        { eauto. }
+        { eauto. }
+        { instantiate (1:=val). etrans; eauto.
+          ss. rewrite <- H1 in *. auto.
+        }
+        { auto. }
+        i. des.
+        esplits.
+        { refl. }
+        { eapply Local.step_read; eauto. }
+        { ss. }
+        { ss. destruct ord; ss. }
+        { i. econs; eauto. }
+      }
+    }
+    { inv LIFT. ss. hexploit (VALS loc); eauto. i. inv H.
+      { hexploit sim_thread_src_write_na_racy; eauto.
+        i. des. esplits.
+        { refl. }
+        { eapply Local.step_racy_write; eauto. }
+        { ss. }
+        { ss. destruct ord; ss. }
+        { ss. }
+      }
+      { hexploit sim_thread_src_write_na; eauto.
+        i. des. esplits.
+        { eauto. }
+        { eapply Local.step_write_na; eauto. }
+        { ss. }
+        { ss. destruct ord; ss. }
+        { i. econs; eauto.
+          { ss. unfold ValueMap.write. ii. des_ifs.
+            { rewrite <- H1. rewrite <- H5. econs; eauto. refl. }
+            { eapply VALS; auto. }
+          }
+          { ss. unfold Flags.update. ii. des_ifs.
+            econs; eauto.
+            { eapply FLAGS; eauto. }
+            { eapply FLAGS; eauto. }
+          }
+          { i. ss. des_ifs.
+            { exfalso. eapply LOCDISJOINT; eauto. }
+            { eapply ATLOCS; eauto. }
+          }
+        }
+      }
+    }
+    { inv LIFT. esplits.
+      { refl. }
+      { eapply Local.step_failure. econs.
+        inv SIM. eapply sim_local_consistent; eauto.
+      }
+      { ss. }
+      { ss. }
+      { ss. }
+    }
+    { inv LIFT. esplits.
+      { refl. }
+      { instantiate (4:=ThreadEvent.racy_update loc valr valw ordr ordw).
+        inv SIM. eapply sim_local_consistent in CONSISTENT; eauto.
+        eapply Local.step_racy_update. red in ORD. des.
+        { econs 1; eauto. }
+        { econs 2; eauto. }
+      }
+      { ss. }
+      { ss. }
+      { ss. }
+    }
+  Qed.
+
+  Lemma sim_lift_src_na_step:
+    forall
+      w p D smem_src0 smem_tgt mem_src0 mem_tgt lc_src0 lc_tgt sc_src0 sc_tgt
+      me smem_src1
+      lang_src st_src0 st_src1
+      (LIFT: sim_state_lift w smem_src0 smem_tgt p D mem_src0 mem_tgt lc_src0 lc_tgt sc_src0 sc_tgt)
+      (STEP: SeqState.na_step p me (SeqState.mk _ st_src0 smem_src0) (SeqState.mk _ st_src1 smem_src1))
+      (NOMIX: nomix _ st_src0)
+      (CONSISTENT: Local.promise_consistent lc_tgt)
+      (WF_SRC: Local.wf lc_src0 mem_src0)
+      (WF_TGT: Local.wf lc_tgt mem_tgt)
+      (SC_SRC: Memory.closed_timemap sc_src0 mem_src0)
+      (SC_TGT: Memory.closed_timemap sc_tgt mem_tgt)
+      (MEM_SRC: Memory.closed mem_src0)
+      (MEM_TGT: Memory.closed mem_tgt),
+    exists lc_src1 mem_src1 sc_src1 lc_src2 mem_src2 sc_src2 e pf,
+      (<<STEPS: rtc (@Thread.tau_step lang_src) (Thread.mk _ st_src0 lc_src0 sc_src0 mem_src0) (Thread.mk _ st_src0 lc_src1 sc_src1 mem_src1)>>) /\
+        (<<STEP: Thread.step pf e (Thread.mk _ st_src0 lc_src1 sc_src1 mem_src1) (Thread.mk _ st_src1 lc_src2 sc_src2 mem_src2)>>) /\
+        (<<MACHINE: ThreadEvent.get_machine_event e = me>>) /\
+        (<<LIFT: forall (NORMAL: ThreadEvent.get_machine_event e <> MachineEvent.failure),
+            sim_state_lift w smem_src1 smem_tgt p D mem_src2 mem_tgt lc_src2 lc_tgt sc_src2 sc_tgt>>) /\
+        (<<NOMIX: nomix _ st_src1>>)
+  .
+  Proof.
+    i. inv STEP.
+    punfold NOMIX. exploit NOMIX; eauto. i. des.
+    hexploit sim_lift_src_na_local_step; eauto.
+    { inv LOCAL; ss.
+      { destruct ord; ss. }
+      { destruct ord; ss. }
+      { red in ORD. des; destruct ordr, ordw; ss. }
+    }
+    { i. eapply NA; eauto. inv LOCAL; ss.
+      { destruct ord; ss. }
+      { destruct ord; ss. }
+      { red in ORD. destruct ordr, ordw; des; ss. }
+    }
+    i. des. subst. esplits; eauto.
+    { econs 2. econs; eauto. }
+    { pclearbot. auto. }
+  Qed.
+
+  Lemma sim_lift_src_na_opt_step:
+    forall
+      w p D smem_src0 smem_tgt mem_src0 mem_tgt lc_src0 lc_tgt sc_src0 sc_tgt
+      me smem_src1
+      lang_src st_src0 st_src1
+      (LIFT: sim_state_lift w smem_src0 smem_tgt p D mem_src0 mem_tgt lc_src0 lc_tgt sc_src0 sc_tgt)
+      (STEP: SeqState.na_opt_step p me (SeqState.mk _ st_src0 smem_src0) (SeqState.mk _ st_src1 smem_src1))
+      (NOMIX: nomix _ st_src0)
+      (CONSISTENT: Local.promise_consistent lc_tgt)
+      (WF_SRC: Local.wf lc_src0 mem_src0)
+      (WF_TGT: Local.wf lc_tgt mem_tgt)
+      (SC_SRC: Memory.closed_timemap sc_src0 mem_src0)
+      (SC_TGT: Memory.closed_timemap sc_tgt mem_tgt)
+      (MEM_SRC: Memory.closed mem_src0)
+      (MEM_TGT: Memory.closed mem_tgt),
+    exists lc_src1 mem_src1 sc_src1 lc_src2 mem_src2 sc_src2 e,
+      (<<STEPS: rtc (@Thread.tau_step lang_src) (Thread.mk _ st_src0 lc_src0 sc_src0 mem_src0) (Thread.mk _ st_src0 lc_src1 sc_src1 mem_src1)>>) /\
+        (<<STEP: Thread.opt_step e (Thread.mk _ st_src0 lc_src1 sc_src1 mem_src1) (Thread.mk _ st_src1 lc_src2 sc_src2 mem_src2)>>) /\
+        (<<MACHINE: ThreadEvent.get_machine_event e = me>>) /\
+        (<<LIFT: forall (NORMAL: ThreadEvent.get_machine_event e <> MachineEvent.failure),
+            sim_state_lift w smem_src1 smem_tgt p D mem_src2 mem_tgt lc_src2 lc_tgt sc_src2 sc_tgt>>) /\
+        (<<NOMIX: nomix _ st_src1>>)
+  .
+  Proof.
+    i. inv STEP.
+    { hexploit sim_lift_src_na_step; eauto.
+      i. des. esplits; eauto. econs 2; eauto.
+    }
+    { esplits; eauto.
+      { econs 1. }
+      { ss. }
+    }
+  Qed.
+
+  Lemma sim_lift_src_na_steps:
+    forall
+      lang_src st_src0 st_src1
+      p smem_src0 smem_src1
+      (STEPS: rtc (SeqState.na_step p MachineEvent.silent) (SeqState.mk _ st_src0 smem_src0) (SeqState.mk _ st_src1 smem_src1))
+      w D smem_tgt mem_src0 mem_tgt lc_src0 lc_tgt sc_src0 sc_tgt
+      (LIFT: sim_state_lift w smem_src0 smem_tgt p D mem_src0 mem_tgt lc_src0 lc_tgt sc_src0 sc_tgt)
+      (NOMIX: nomix _ st_src0)
+      (CONSISTENT: Local.promise_consistent lc_tgt)
+      (WF_SRC: Local.wf lc_src0 mem_src0)
+      (WF_TGT: Local.wf lc_tgt mem_tgt)
+      (SC_SRC: Memory.closed_timemap sc_src0 mem_src0)
+      (SC_TGT: Memory.closed_timemap sc_tgt mem_tgt)
+      (MEM_SRC: Memory.closed mem_src0)
+      (MEM_TGT: Memory.closed mem_tgt),
+    exists lc_src1 mem_src1 sc_src1,
+      (<<STEPS: rtc (@Thread.tau_step lang_src) (Thread.mk _ st_src0 lc_src0 sc_src0 mem_src0) (Thread.mk _ st_src1 lc_src1 sc_src1 mem_src1)>>) /\
+        (<<LIFT: sim_state_lift w smem_src1 smem_tgt p D mem_src1 mem_tgt lc_src1 lc_tgt sc_src1 sc_tgt>>) /\
+        (<<NOMIX: nomix _ st_src1>>)
+  .
+  Proof.
+    intros lang_src st_src0 st_src1 p smem_src0 smem_src1 STEPS.
+    remember (SeqState.mk _ st_src0 smem_src0) as th_src0.
+    remember (SeqState.mk _ st_src1 smem_src1) as th_src1.
+    revert st_src0 st_src1 smem_src0 smem_src1 Heqth_src0 Heqth_src1.
+    induction STEPS; i; clarify.
+    { esplits.
+      { refl. }
+      { auto. }
+      { auto. }
+    }
+    destruct y. hexploit sim_lift_src_na_step; eauto. i. des.
+    hexploit Thread.rtc_tau_step_future; eauto. i. des; ss.
+    hexploit Thread.step_future; eauto. i. des; ss.
+    hexploit LIFT0; eauto.
+    { rewrite MACHINE. ss. }
+    i. hexploit IHSTEPS; eauto. i. des. esplits.
+    { etrans; [eauto|]. econs.
+      { econs; eauto. econs; eauto. }
+      { eauto. }
+    }
+    { eauto. }
+    { eauto. }
+  Qed.
+
+  Variant sim_val_sol_lift: forall (p: Perm.t) (P: bool) (sv: Const.t) (v: Const.t), Prop :=
+    | sim_val_sol_lift_high
+        sv v
+        (VAL: Const.le sv v)
+      :
+      sim_val_sol_lift Perm.high true sv v
+    | sim_val_sol_lift_low
+        sv v
+      :
+      sim_val_sol_lift Perm.low false sv v
+  .
+
+  Definition sim_vals_sol_lift (p: Perms.t) (P: Loc.t -> bool) (svs: ValueMap.t) (vs: Loc.t -> Const.t) :=
+    forall loc (NA: loc_na loc), sim_val_sol_lift (p loc) (P loc) (svs loc) (vs loc).
+
+  Variant sim_flag_sol_lift (D: Flag.t) (d: bool) (W: Flag.t) (flag: Flag.t): Prop :=
+    | sim_flag_sol_lift_intro
+        (DEBT: d -> D)
+        (SS: Flag.join W flag -> ~ d)
+  .
+
+  Definition sim_flags_sol_lift (D: Flags.t) (d: Loc.t -> bool) (W: Flags.t) (flag: Flags.t): Prop :=
+    forall loc (NA: loc_na loc), sim_flag_sol_lift (D loc) (d loc) (W loc) (flag loc).
+
+  Variant sim_state_sol_lift (c: bool):
+    forall (smem: SeqMemory.t) (p: Perms.t) (D: Flags.t) (W: Flags.t)
+           (mem: Memory.t) (lc: Local.t) (sc: TimeMap.t) (o: Oracle.t), Prop :=
+    | sim_state_sol_lift_intro
+        svs flag
+        p P W d D vs ovs
+        mem lc sc
+        (SIM: sim_thread_sol c vs P d mem lc)
+        (VAL: sim_vals_sol_lift p P svs vs)
+        (FLAG: sim_flags_sol_lift D d W flag)
+        (OVALS: forall loc (NA: loc_at loc), ovs loc = vs loc)
+      :
+      sim_state_sol_lift
+        c
+        (SeqMemory.mk svs flag)
+        p D W
+        mem lc sc (CertOracle.to_oracle ovs)
+  .
+
+  Lemma sim_lift_sim_lift_sol c:
+    forall
+      w p D smem_src smem_tgt mem_src0 mem_tgt lc_src0 lc_tgt sc_src0 sc_tgt
+      lang_src st_src
+      (LIFT: sim_state_lift w smem_src smem_tgt p D mem_src0 mem_tgt lc_src0 lc_tgt sc_src0 sc_tgt)
+      (CONSISTENT: Local.promise_consistent lc_tgt)
+      (WF_SRC: Local.wf lc_src0 mem_src0)
+      (WF_TGT: Local.wf lc_tgt mem_tgt)
+      (SC_SRC: Memory.closed_timemap sc_src0 mem_src0)
+      (SC_TGT: Memory.closed_timemap sc_tgt mem_tgt)
+      (MEM_SRC: Memory.closed mem_src0)
+      (MEM_TGT: Memory.closed mem_tgt)
+      (CERTIFIED: c = true -> lc_tgt.(Local.promises) = Memory.bot),
+    exists lc_src1 mem_src1 sc_src1 o,
+      (<<STEPS: rtc (@Thread.tau_step lang_src) (Thread.mk _ st_src lc_src0 sc_src0 mem_src0) (Thread.mk _ st_src lc_src1 sc_src1 mem_src1)>>) /\
+        (<<LIFT: sim_state_sol_lift
+                   c smem_src p (Flags.join D smem_tgt.(SeqMemory.flags)) smem_src.(SeqMemory.flags) mem_src1 lc_src1 sc_src1 o>>).
+  Proof.
+    i. inv LIFT.
+    hexploit sim_thread_sim_thread_sol; eauto.
+    { instantiate (1:=fun loc => Flag.minus (flag_tgt loc) (flag_src loc)).
+      i. ss. destruct (flag_src loc), (flag_tgt loc); ss.
+    }
+    i. des. esplits; eauto.
+    econs; eauto.
+    { ii. hexploit (VALS loc); eauto. i. inv H.
+      { econs; eauto. }
+      { hexploit VALS0; eauto. i. rewrite H. econs; eauto. }
+    }
+    { ii. ss. hexploit (FLAGS loc); eauto. i. inv H. econs.
+      { unfold Flags.minus, Flags.join.
+        destruct (D loc), (sflag_tgt loc), (sflag_src loc), (flag_tgt loc), (flag_src loc); auto.
+      }
+      { unfold Flags.minus, Flags.join. ii.
+        destruct (D loc), (sflag_tgt loc), (sflag_src loc), (flag_tgt loc), (flag_src loc); ss.
+      }
+    }
+  Qed.
+
+  Lemma sim_lift_na_local_step c:
+    forall
+      p D W smem0 mem0 lc0 sc0 o
+      smem1 me pe
+      (LIFT: sim_state_sol_lift c smem0 p D W mem0 lc0 sc0 o)
+      (STEP: SeqState.na_local_step p me pe smem0 smem1)
+      (NALOCS: forall loc val (ACCESS: is_accessing pe = Some (loc, val)), loc_na loc)
+      (WF_SRC: Local.wf lc0 mem0)
+      (SC_SRC: Memory.closed_timemap sc0 mem0)
+      (MEM_SRC: Memory.closed mem0)
+      lang st,
+    exists lc1 mem1 sc1 lc2 mem2 sc2 e,
+      (<<STEPS: rtc (@Thread.tau_step lang) (Thread.mk _ st lc0 sc0 mem0) (Thread.mk _ st lc1 sc1 mem1)>>) /\
+        (<<STEP: Local.program_step e lc1 sc1 mem1 lc2 sc2 mem2>>) /\
+        (<<MACHINE: ThreadEvent.get_machine_event e = me \/ ThreadEvent.get_machine_event e = MachineEvent.failure>>) /\
+        (<<EVENT: ThreadEvent.get_program_event e = pe>>) /\
+        (<<LIFT: forall (NORMAL: ThreadEvent.get_machine_event e <> MachineEvent.failure),
+            sim_state_sol_lift c smem1 p D W mem2 lc2 sc2 o>>).
+  Proof.
+    i. inv STEP.
+    { esplits.
+      { refl. }
+      { eapply Local.step_silent. }
+      { eauto. }
+      { eauto. }
+      { eauto. }
+    }
+    { inv LIFT. destruct ord; ss.
+      hexploit (VAL0 loc); eauto. i. inv H.
+      { rewrite <- H1 in *.
+        hexploit sim_thread_sol_read_na.
+        { eauto. }
+        { eauto. }
+        { etrans; [eapply VAL; auto|eapply VAL1]. }
+        i. des. esplits.
+        { refl. }
+        { eapply Local.step_read; eauto. }
+        { eauto. }
+        { ss. }
+        { i. econs; eauto. }
+      }
+      { rewrite <- H1 in *.
+        hexploit sim_thread_sol_read_na_racy; eauto.
+        { rewrite <- H2. ss. }
+        i. des. esplits.
+        { refl. }
+        { eapply Local.step_racy_read; eauto. }
+        { eauto. }
+        { ss. }
+        { i. econs; eauto. }
+      }
+    }
+    { inv LIFT. destruct ord; ss.
+      hexploit (VAL loc); eauto. i. inv H.
+      { hexploit sim_thread_sol_write_na; eauto. i. des.
+        { esplits.
+          { refl. }
+          { eapply Local.step_racy_write; eauto. }
+          { eauto. }
+          { ss. }
+          { ss. }
+        }
+        { esplits.
+          { eauto. }
+          { eapply Local.step_write_na; eauto. }
+          { eauto. }
+          { ss. }
+          { i. econs; eauto.
+            { ii. unfold ValueMap.write. ss. des_ifs.
+              { rewrite <- H1. econs. refl. }
+              { eapply VAL; auto. }
+            }
+            { ii. unfold Flags.update. ss. des_ifs.
+              eapply FLAG; auto.
+            }
+            { i. ss. des_ifs.
+              { exfalso. eapply LOCDISJOINT; eauto. }
+              { eapply OVALS; eauto. }
+            }
+          }
+        }
+      }
+      { hexploit sim_thread_sol_write_na_racy; eauto.
+        { rewrite <- H2. ss. }
+        i. des. esplits.
+        { refl. }
+        { eapply Local.step_racy_write; eauto. }
+        { eauto. }
+        { ss. }
+        { ss. }
+      }
+    }
+    { inv LIFT. hexploit sim_thread_sol_failure; eauto. i.
+      esplits.
+      { refl. }
+      { eapply Local.step_failure; eauto. }
+      { eauto. }
+      { ss. }
+      { ss. }
+    }
+    { inv LIFT. esplits.
+      { refl. }
+      { eapply Local.step_racy_update.
+        instantiate (1:=ordw). instantiate (1:=ordr).
+        red in ORD. des.
+        { econs 1; eauto. inv SIM. auto. }
+        { econs 2; eauto. inv SIM. auto. }
+      }
+      { auto. }
+      { ss. }
+      { ss. }
+    }
+  Qed.
+
+        failure; eauto. }
+      { eauto. }
+      { ss. }
+      { ss. }
+    }
+
+
+      sim_thread_failure; eauto.
+
+
+        }
+        { esplits.
+          { eauto. }
+          { eapply Local.step_write_na; eauto. }
+          { eauto. }
+          { ss. }
+          { i. econs; eauto.
+            { ii. unfold ValueMap.write. ss. des_ifs.
+              { rewrite <- H1. econs. refl. }
+              { eapply VAL; auto. }
+            }
+            { ii. unfold Flags.update. ss. des_ifs.
+              eapply FLAG; auto.
+            }
+            { i. ss. des_ifs.
+              { exfalso. eapply LOCDISJOINT; eauto. }
+              { eapply OVALS; eauto. }
+            }
+          }
+        }
+      }
+
+            }
+
+
+              eapply
+
+            { eauto.
+
+            ss. }
+        }
+
+        sim_thread_sol _read_na.
+        { eauto. }
+        { eauto. }
+        { etrans; [eapply VAL; auto|eapply VAL1]. }
+        i. des. esplits.
+        { refl. }
+        { eapply Local.step_read; eauto. }
+        { eauto. }
+        { ss. }
+        { i. econs; eauto. }
+      }
+      { rewrite <- H1 in *.
+        hexploit sim_thread_sol_read_na_racy; eauto.
+        { rewrite <- H2. ss. }
+        i. des. esplits.
+        { refl. }
+        { eapply Local.step_racy_read; eauto. }
+        { eauto. }
+        { ss. }
+        { i. econs; eauto. }
+      }
+    }
+
+        ss.
+
+
+        destruct ord; ss. eauto. }
+        { eauto. }
+        {
+
+
+      destruct
+
+      esplits.
+      { refl. }
+      { eapply Local.step_silent. }
+      { eauto. }
+      { eauto. }
+      { eauto. }
+    }
+
+
+            sim_state_lift w smem_src1 smem_tgt p D mem_src2 mem_tgt lc_src2 lc_tgt sc_src2 sc_tgt>>)
+
+
+
+      SeqState.na_local_step p e pe smem0 smem1
+
+SeqThread.na_step
+ SeqThread.steps (SeqState.na_step (lang:=lang_src)) tr
+
+
+sim_seq_failure_case
+
+    ,
+    exists lc_src1 mem_src1 sc_src1 o,
+      (<<STEPS: rtc (@Thread.tau_step lang_src) (Thread.mk _ st_src lc_src0 sc_src0 mem_src0) (Thread.mk _ st_src lc_src1 sc_src1 mem_src1)>>) /\
+        (<<LIFT: sim_state_sol_lift c smem p D W mem lc sc o>>)
+
+                   (Flags.join D smem_tgt.(SeqMemory.flags)) smem_src.(SeqMemory.flags) mem_src1 lc_src1 sc_src1 o>>).
+  Proof.
+
+
+
+  Variant sim_flag_lift
+          (d: Flag.t) (sflag_src: Flag.t) (sflag_tgt: Flag.t)
+          (flag_src: option Time.t) (flag_tgt: option Time.t): Prop :=
+    | sim_flag_lift_intro
+        (TGT: d \/ sflag_tgt -> flag_tgt)
+        (SRC: sflag_src <-> flag_src)
+  .
+
+
+
+                                          svs: ValueMap.t) (
+
+             (P: Loc.t -> bool) (svs: ValueMap.t) (vs: Loc.t -> Const.t) :=
+    forall loc, sim_val_sol_lift (p loc) (P loc) (svs loc) (vs loc).
+
+  Definition sim_vals_sol_lift (p: Perms.t) (P: Loc.t -> bool) (svs: ValueMap.t) (vs: Loc.t -> Const.t) :=
+    forall loc, sim_val_sol_lift (p loc) (P loc) (svs loc) (vs loc).
+
+sim_val_lift
+
+
+                f vers flag_src flag_tgt vs_src vs_tgt mem_src mem_tgt lc_src lc_tgt sc_src sc_tgt)
+        (VALS: sim_vals_lift p svs_src svs_tgt vs_src vs_tgt)
+        (FLAGS: sim_flags_lift D sflag_src sflag_tgt flag_src flag_tgt)
+        (WF: Mapping.wfs f)
+        (VERS: versions_wf f vers)
+        (VERSIONED: versioned_memory vers mem_tgt)
+      :
+      sim_state_lift
+        (f, vers, mem_tgt)
+        (SeqMemory.mk svs_src sflag_src) (SeqMemory.mk svs_tgt sflag_tgt)
+        p D
+        mem_src mem_tgt lc_src lc_tgt sc_src sc_tgt
+  .
+
+  sim_seq_partial_case
+  SeqThread.
+
+  Variant sim_state_sol_lift: forall
+      (p: Perm.t)
+      (sv_src: Const.t) (sv_tgt: Const.t)
+      (v_src: option Const.t) (v_tgt: option Const.t), Prop :=
+    | sim_val_lift_low
+        sv_src sv_tgt
+      :
+      sim_val_lift Perm.low sv_src sv_tgt None None
+    | sim_val_lift_high
+        sv_src sv_tgt v_src v_tgt
+        (VALSRC: Const.le sv_src v_src)
+        (VALTGT: Const.le v_tgt sv_tgt)
+      :
+      sim_val_lift Perm.high sv_src sv_tgt (Some v_src) (Some v_tgt)
+  .
+
+  c vs P D mem lc
+
+    (sim
+
+  sim_thread_sol
+
+  Lemma sim_lift_sol_na_step:
+    forall
+      lang_src st_src0 st_src1
+      p smem_src0 smem_src1
+      (STEPS: rtc (SeqState.na_step p MachineEvent.silent) (SeqState.mk _ st_src0 smem_src0) (SeqState.mk _ st_src1 smem_src1))
+      w D smem_tgt mem_src0 mem_tgt lc_src0 lc_tgt sc_src0 sc_tgt
+      (LIFT: sim_state_lift w smem_src0 smem_tgt p D mem_src0 mem_tgt lc_src0 lc_tgt sc_src0 sc_tgt)
+      (CONSISTENT: Local.promise_consistent lc_tgt)
+      (WF_SRC: Local.wf lc_src0 mem_src0)
+      (WF_TGT: Local.wf lc_tgt mem_tgt)
+      (SC_SRC: Memory.closed_timemap sc_src0 mem_src0)
+      (SC_TGT: Memory.closed_timemap sc_tgt mem_tgt)
+      (MEM_SRC: Memory.closed mem_src0)
+      (MEM_TGT: Memory.closed mem_tgt),
+    exists lc_src1 mem_src1 sc_src1,
+      (<<STEPS: rtc (@Thread.tau_step lang_src) (Thread.mk _ st_src0 lc_src0 sc_src0 mem_src0) (Thread.mk _ st_src1 lc_src1 sc_src1 mem_src1)>>) /\
+        (<<LIFT: sim_state_lift w smem_src1 smem_tgt p D mem_src1 mem_tgt lc_src1 lc_tgt sc_src1 sc_tgt>>)
+  .
+  Proof.
+    intros lang_src st_src0 st_src1 p smem_src0 smem_src1 STEPS.
+    remember (SeqState.mk _ st_src0 smem_src0) as th_src0.
+    remember (SeqState.mk _ st_src1 smem_src1) as th_src1.
+    revert st_src0 st_src1 smem_src0 smem_src1 Heqth_src0 Heqth_src1.
+    induction STEPS; i; clarify.
+    { esplits.
+      { refl. }
+      { auto. }
+    }
+    destruct y. hexploit sim_lift_src_na_step; eauto. i. des.
+    hexploit Thread.rtc_tau_step_future; eauto. i. des; ss.
+    hexploit Thread.step_future; eauto. i. des; ss.
+    hexploit LIFT0; eauto.
+    { rewrite MACHINE. ss. }
+    i. hexploit IHSTEPS; eauto. i. des. esplits.
+    { etrans; [eauto|]. econs.
+      { econs; eauto. econs; eauto. }
+      { eauto. }
+    }
+    { eauto. }
+  Qed.
+
+  sim_thread_sole
+
+
+  Definition sim_vals_lift
+             (p: Perms.t) (svs_src: ValueMap.t) (svs_tgt: ValueMap.t)
+             (vs_src: Loc.t -> option Const.t) (vs_tgt: Loc.t -> option Const.t): Prop :=
+    forall loc, sim_val_lift (p loc) (svs_src loc) (svs_tgt loc) (vs_src loc) (vs_tgt loc).
+
+  Variant sim_flag_lift
+          (d: Flag.t) (sflag_src: Flag.t) (sflag_tgt: Flag.t)
+          (flag_src: option Time.t) (flag_tgt: option Time.t): Prop :=
+    | sim_flag_lift_intro
+        (TGT: d \/ sflag_tgt -> flag_tgt)
+        (SRC: sflag_src <-> flag_src)
+  .
+
+  Definition sim_flags_lift
+             (d: Flags.t) (sflag_src: Flags.t) (sflag_tgt: Flags.t)
+             (flag_src: Loc.t -> option Time.t) (flag_tgt: Loc.t -> option Time.t): Prop :=
+    forall loc, sim_flag_lift (d loc) (sflag_src loc) (sflag_tgt loc) (flag_src loc) (flag_tgt loc).
+
+  Variant sim_state_lift:
+    forall (w: world)
+           (smem_src: SeqMemory.t) (smem_tgt: SeqMemory.t)
+           (p: Perms.t)
+           (D: Flags.t)
+           (mem_src: Memory.t)
+           (mem_tgt: Memory.t)
+           (lc_src: Local.t)
+           (lc_tgt: Local.t)
+           (sc_src: TimeMap.t)
+           (sc_tgt: TimeMap.t), Prop :=
+    | sim_state_lift_intro
+        svs_src sflag_src svs_tgt sflag_tgt
+        p D f vers flag_src flag_tgt vs_src vs_tgt
+        mem_src mem_tgt lc_src lc_tgt sc_src sc_tgt
+        (SIM: SeqLiftStep.sim_thread f vers flag_src flag_tgt vs_src vs_tgt mem_src mem_tgt lc_src lc_tgt sc_src sc_tgt)
+        (VALS: sim_vals_lift p svs_src svs_tgt vs_src vs_tgt)
+        (FLAGS: sim_flags_lift D sflag_src sflag_tgt flag_src flag_tgt)
+        (WF: Mapping.wfs f)
+        (VERS: versions_wf f vers)
+        (VERSIONED: versioned_memory vers mem_tgt)
+      :
+      sim_state_lift
+        (f, vers, mem_tgt)
+        (SeqMemory.mk svs_src sflag_src) (SeqMemory.mk svs_tgt sflag_tgt)
+        p D
+        mem_src mem_tgt lc_src lc_tgt sc_src sc_tgt
+  .
+
+
+  sim_thread_sole
+
+
+  SeqThread.steps (SeqState.na_step (lang:=lang_src)) tr
+    {| SeqThread.state := st_src0; SeqThread.perm := p0; SeqThread.oracle := o |} th >> /\
+  << SeqThread.writing_trace tr w >> /\ << SeqThread.failure (SeqState.na_step (lang:=lang_src)) th >>
+
+
+  sim_seq_failure_case
+
+  Lemma sim_lift_sole_step:
+    forall
+      lang_src st_src0 st_src1
+      p smem_src0 smem_src1
+      (STEPS: rtc (SeqState.na_step p MachineEvent.silent) (SeqState.mk _ st_src0 smem_src0) (SeqState.mk _ st_src1 smem_src1))
+      w D smem_tgt mem_src0 mem_tgt lc_src0 lc_tgt sc_src0 sc_tgt
+      (LIFT: sim_state_lift w smem_src0 smem_tgt p D mem_src0 mem_tgt lc_src0 lc_tgt sc_src0 sc_tgt)
+      (CONSISTENT: Local.promise_consistent lc_tgt)
+      (WF_SRC: Local.wf lc_src0 mem_src0)
+      (WF_TGT: Local.wf lc_tgt mem_tgt)
+      (SC_SRC: Memory.closed_timemap sc_src0 mem_src0)
+      (SC_TGT: Memory.closed_timemap sc_tgt mem_tgt)
+      (MEM_SRC: Memory.closed mem_src0)
+      (MEM_TGT: Memory.closed mem_tgt),
+    exists lc_src1 mem_src1 sc_src1,
+      (<<STEPS: rtc (@Thread.tau_step lang_src) (Thread.mk _ st_src0 lc_src0 sc_src0 mem_src0) (Thread.mk _ st_src1 lc_src1 sc_src1 mem_src1)>>) /\
+        (<<LIFT: sim_state_lift w smem_src1 smem_tgt p D mem_src1 mem_tgt lc_src1 lc_tgt sc_src1 sc_tgt>>)
+  .
+  Proof.
+    intros lang_src st_src0 st_src1 p smem_src0 smem_src1 STEPS.
+    remember (SeqState.mk _ st_src0 smem_src0) as th_src0.
+    remember (SeqState.mk _ st_src1 smem_src1) as th_src1.
+    revert st_src0 st_src1 smem_src0 smem_src1 Heqth_src0 Heqth_src1.
+    induction STEPS; i; clarify.
+    { esplits.
+      { refl. }
+      { auto. }
+    }
+    destruct y. hexploit sim_lift_src_na_step; eauto. i. des.
+    hexploit Thread.rtc_tau_step_future; eauto. i. des; ss.
+    hexploit Thread.step_future; eauto. i. des; ss.
+    hexploit LIFT0; eauto.
+    { rewrite MACHINE. ss. }
+    i. hexploit IHSTEPS; eauto. i. des. esplits.
+    { etrans; [eauto|]. econs.
+      { econs; eauto. econs; eauto. }
+      { eauto. }
+    }
+    { eauto. }
+  Qed.
+
+
+
+CertOracle
+
+  Oracle.t
+
+
+sim_seq_na_step_case =
+fun (lang_src lang_tgt : language)
+  (sim_seq : Perms.t -> Flags.t -> SeqState.t lang_src -> SeqState.t lang_tgt -> Prop)
+  (p0 : Perms.t) (d0 : Flags.t) (st_src0 : SeqState.t lang_src) (st_tgt0 : SeqState.t lang_tgt) =>
+forall (st_tgt1 : SeqState.t lang_tgt) (e : MachineEvent.t),
+SeqState.na_step p0 e st_tgt0 st_tgt1 ->
+exists st_src1 st_src2 : SeqState.t lang_src,
+  << rtc (SeqState.na_step p0 MachineEvent.silent) st_src0 st_src1 >> /\
+  << SeqState.na_opt_step p0 e st_src1 st_src2 >> /\ << sim_seq p0 d0 st_src2 st_tgt1 >>
+     : forall lang_src lang_tgt : language,
+       (Perms.t -> Flags.t -> SeqState.t lang_src -> SeqState.t lang_tgt -> Prop) ->
+       Perms.t -> Flags.t -> SeqState.t lang_src -> SeqState.t lang_tgt -> Prop
+
+
+
+    sim_seq_normal : sim_seq_terminal_case sim_terminal p0 d0 st_src0 st_tgt0 ->
+                     sim_seq_na_step_case (sim_seq lang_src lang_tgt sim_terminal) p0 d0 st_src0 st_tgt0 ->
+                     sim_seq_at_step_case (sim_seq lang_src lang_tgt sim_terminal) p0 d0 st_src0 st_tgt0 ->
+                     sim_seq_partial_case p0 d0 st_src0 st_tgt0 ->
+                     _sim_seq sim_seq sim_terminal p0 d0 st_src0 st_tgt0
+
+
+  _sim_seq
+
+      (EVENT: ThreadEvent.get_program_event e = pe)
+      (NA: ~ is_atomic_event pe)
+      (LOWER: is_na_write e -> mem_tgt1 = mem_tgt0)
+
+
+
+              (* (<<EVENT: me = MachineEvent.failure ->  *)
+
+        (<<STEP: Local.program_step SeqState.na_local_step p me pe smem_tgt0 smem_tgt1>>) /\
+        (<<LIFT: forall (NORMAL: me <> MachineEvent.failure),
+            sim_state_lift w smem_src smem_tgt1 p D mem_src1 mem_tgt1 lc_src1 lc_tgt1 sc_src1 sc_tgt1>>)
+  .
+
+    Thread.program_step
+
+
+      (STEP: Local.program_step e lc_tgt0 sc_tgt0 mem_tgt0 lc_tgt1 sc_tgt1 mem_tgt1)
+      (EVENT: ThreadEvent.get_program_event e = pe)
+      (NA: ~ is_atomic_event pe)
+      (LOWER: is_na_write e -> mem_tgt1 = mem_tgt0)
+
+      (CONSISTENT: Local.promise_consistent lc_tgt1)
+      (WF_SRC: Local.wf lc_src0 mem_src0)
+      (WF_TGT: Local.wf lc_tgt0 mem_tgt0)
+      (SC_SRC: Memory.closed_timemap sc_src0 mem_src0)
+      (SC_TGT: Memory.closed_timemap sc_tgt0 mem_tgt0)
+      (MEM_SRC: Memory.closed mem_src0)
+      (MEM_TGT: Memory.closed mem_tgt0)
+      lang_src st_src,
+    exists lc_src1 mem_src1 sc_src1 me smem_tgt1,
+      (<<STEPS: rtc (@Thread.tau_step lang_src) (Thread.mk _ st_src lc_src0 sc_src0 mem_src0) (Thread.mk _ st_src lc_src1 sc_src1 mem_src1)>>) /\
+      (<<STEP: SeqState.na_local_step p me pe smem_tgt0 smem_tgt1>>) /\
+        (<<LIFT: forall (NORMAL: me <> MachineEvent.failure),
+            sim_state_lift w smem_src smem_tgt1 p D mem_src1 mem_tgt1 lc_src1 lc_tgt1 sc_src1 sc_tgt1>>)
+  .
+  Proof.
+    i. inv STEP; ss.
+    { esplits.
+      { refl. }
+      { econs 1. }
+      { eauto. }
+    }
+    { inv LIFT. destruct ord; ss. hexploit sim_thread_tgt_read_na; eauto.
+      i. des. esplits.
+      { refl. }
+      { econs 2; eauto. i. ss. specialize (VALS loc). inv VALS.
+        { des_ifs. }
+        hexploit VAL; eauto. i. etrans; eauto.
+      }
+      { i. econs; eauto. }
+    }
+    { destruct ord; ss. eapply local_write_step_write_na_step in LOCAL.
+      eapply sim_lift_tgt_na_write_step; eauto.
+    }
+    { esplits.
+      { refl. }
+      { econs 5. red. destruct ordr, ordw; ss; auto. }
+      { ss. }
+    }
+    { esplits.
+      { refl. }
+      { econs 4. }
+      { ss. }
+    }
+    { destruct ord; ss. eapply sim_lift_tgt_na_write_step; eauto. }
+    { inv LIFT. destruct ord; ss. hexploit sim_thread_tgt_read_na_racy; eauto.
+      i. esplits.
+      { refl. }
+      { econs 2; eauto. i. specialize (VALS loc). rewrite H in VALS. inv VALS.
+        rewrite <- H2 in *. ss.
+      }
+      { i. econs; eauto. }
+    }
+    { inv LIFT. destruct ord; ss. hexploit sim_thread_tgt_write_na_racy; eauto.
+      i. esplits.
+      { refl. }
+      { econs 3; eauto. }
+      { i. specialize (VALS loc). rewrite H in VALS. inv VALS.
+        rewrite <- H1 in *. ss.
+      }
+    }
+    { esplits.
+      { refl. }
+      { econs 5. red. destruct ordr, ordw; ss; auto. }
+      { ss. }
+    }
+  Qed.
+
+
+    {
+
+      { i. econs; eauto. }
+
+    }}
+   {
+
+      eauto.
+
+      hexploit sim_thread_tgt_racy_read; eauto.
+      i. des. esplits.
+      { refl. }
+      { econs 2; eauto. i. ss. specialize (VALS loc). inv VALS.
+        { des_ifs. }
+        hexploit VAL; eauto. i. etrans; eauto.
+      }
+      { i. econs; eauto. }
+    }
+
+
+    {
+
+    }
+    {
+
+
+    { destruct ord; ss. hexploit sim_thread_tgt_read_na; eauto.
+      i. des. esplits.
+      { econs 2; eauto. i. ss. specialize (VALS loc). inv VALS.
+        { des_ifs. }
+        hexploit VAL; eauto. i. etrans; eauto.
+      }
+      { econs; eauto. }
+    }
+
+
+
+      esplits.
+
+      esplits; eauto.
+
+      sim_thread_tgt_read_na:
+  forall (f : Mapping.ts) (vers : versions) (flag_src flag_tgt : Loc.t -> option Time.t)
+    (vs_src vs_tgt : Loc.t -> option Const.t) (mem_src mem_tgt : Memory.t) (lc_src lc_tgt0 : Local.t)
+    (sc_src sc_tgt : TimeMap.t) (loc : Loc.t) (to_tgt : Time.t) (val_tgt : Const.t)
+    (vw_tgt : option View.t) (lc_tgt1 : Local.t),
+  Local.read_step lc_tgt0 mem_tgt loc to_tgt val_tgt vw_tgt Ordering.na lc_tgt1 ->
+  SeqLiftStep.sim_thread f vers flag_src flag_tgt vs_src vs_tgt mem_src mem_tgt lc_src lc_tgt0 sc_src sc_tgt ->
+  Local.promise_consistent lc_tgt1 ->
+  Local.wf lc_tgt0 mem_tgt ->
+  Memory.closed mem_tgt ->
+  <<
+  SeqLiftStep.sim_thread f vers flag_src flag_tgt vs_src vs_tgt mem_src mem_tgt lc_src lc_tgt1 sc_src sc_tgt >> /\
+  << forall val : Const.t, vs_tgt loc = Some val -> Const.le val_tgt val >>
+
+
+
+    P
+
+    SeqEvent.t
+      ProgramEvent.t
+
+
+        SeqState.na_local_step p e smem_tgt0 smem_tgt1),
+      (<<FAILURE
+         exists mem
+
+                Thread.program_step
+
+                Local.program_step
+
+
+      :
+
+                                    (Seq.mk
+
+    ,
+      @sim_thread
+        world world_messages_le sim_memory_lift sim_timemap_lift
+        lang_src lang_tgt true w st_src lc_src sc_src mem_src st_tgt lc_tgt sc_tgt mem_tgt.
+  Proof.
+    pcofix CIH. i. inv LIFT. pfold. ii. splits; ss.
+    { admit. }
+    { admit. }
+    { ii. punfold SIM. inv SIM. exploit TERMINAL; eauto. i. ss. des.
+
+
+  Lemma sim_lift_tgt_na_step
+        w p D smem_src smem_tgt mem_src mem_tgt lc_src lc_tgt sc_src sc_tgt
+        (LIFT: sim_state_lift w smem_src smem_tgt p D mem_src mem_tgt lc_src lc_tgt sc_src sc_tgt),
+    @_sim_thread_failure
+      world lang_src lang_tgt w st_src lc_src sc_src mem_src st_tgt lc_tgt sc_tgt mem_tgt.
+  Proof.
+    ii. red in SIM. inv SIM.
+
+    SeqState.t .na_local_step
+
+    | na_local_step_silent
+      m
+    :
+      na_local_step
+        p
+        (MachineEvent.silent) (ProgramEvent.silent)
+        m m
+  | na_local_step_read
+      m
+      loc val ord
+      (ORD: Ordering.le ord Ordering.na)
+      (VAL: Perm.le Perm.high (p loc) -> Const.le val (SeqMemory.read loc m))
+    :
+      na_local_step
+        p
+        (MachineEvent.silent) (ProgramEvent.read loc val ord)
+        m m
+  | na_local_step_write
+      m0 m1 e
+      loc val ord
+      (ORD: Ordering.le ord Ordering.na)
+      (MEM: SeqMemory.write loc val m0 = m1)
+      (PERM: e = if Perm.le Perm.high (p loc) then MachineEvent.silent else MachineEvent.failure)
+    :
+      na_local_step
+        p
+        e (ProgramEvent.write loc val ord)
+        m0 m1
+  | na_local_step_failure
+      m
+    :
+      na_local_step
+        p
+        (MachineEvent.failure) (ProgramEvent.failure)
+        m m
+  | na_local_step_update
+      m
+      loc valr valw ordr ordw
+      (ORD: __guard__(Ordering.le ordr Ordering.na \/ Ordering.le ordw Ordering.na))
+    :
+      na_local_step
+        p
+        (MachineEvent.failure) (ProgramEvent.update loc valr valw ordr ordw)
+        m m
+  .
+
+
+
+  Lemma sim_lift_failure lang_src lang_tgt:
+    forall
+      (st_src: lang_src.(Language.state)) (st_tgt: lang_tgt.(Language.state))
+      w p D smem_src smem_tgt mem_src mem_tgt lc_src lc_tgt sc_src sc_tgt
+      (SIM: sim_seq_failure_case p (SeqState.mk _ st_src smem_src))
+      (LIFT: sim_state_lift w smem_src smem_tgt p D mem_src mem_tgt lc_src lc_tgt sc_src sc_tgt),
+      @_sim_thread_failure
+        world lang_src lang_tgt w st_src lc_src sc_src mem_src st_tgt lc_tgt sc_tgt mem_tgt.
+  Proof.
+    ii. red in SIM. inv SIM.
+
+
+    Variant
+_sim_seq
+    (sim_seq : forall lang_src lang_tgt : language,
+               (Language.state lang_src -> Language.state lang_tgt -> Prop) ->
+               Perms.t ->
+               Flags.t -> SeqState.t lang_src -> SeqState.t lang_tgt -> Prop)
+(lang_src lang_tgt : language)
+(sim_terminal : Language.state lang_src -> Language.state lang_tgt -> Prop)
+(p0 : Perms.t) (d0 : Flags.t) (st_src0 : SeqState.t lang_src)
+(st_tgt0 : SeqState.t lang_tgt) : Prop :=
+    sim_seq_normal : sim_seq_terminal_case sim_terminal p0 d0 st_src0 st_tgt0 ->
+                     sim_seq_na_step_case
+                       (sim_seq lang_src lang_tgt sim_terminal) p0 d0 st_src0
+                       st_tgt0 ->
+                     sim_seq_at_step_case
+                       (sim_seq lang_src lang_tgt sim_terminal) p0 d0 st_src0
+                       st_tgt0 ->
+                     sim_seq_partial_case p0 d0 st_src0 st_tgt0 ->
+                     _sim_seq sim_seq sim_terminal p0 d0 st_src0 st_tgt0
+  | sim_seq_failure : sim_seq_failure_case p0 st_src0 ->
+                      _sim_seq sim_seq sim_terminal p0 d0 st_src0 st_tgt0
+
+
+  Lema
+
+  Lemma sim_lift lang_src lang_tgt sim_terminal:
+    forall
+      (st_src: lang_src.(Language.state)) (st_tgt: lang_tgt.(Language.state))
+      w p D smem_src smem_tgt mem_src mem_tgt lc_src lc_tgt sc_src sc_tgt
+      (SIM: sim_seq sim_terminal p D (SeqState.mk _ st_src smem_src) (SeqState.mk _ st_tgt smem_tgt))
+      (LIFT: sim_state_lift w smem_src smem_tgt p D mem_src mem_tgt lc_src lc_tgt sc_src sc_tgt),
+      @sim_thread
+        world world_messages_le sim_memory_lift sim_timemap_lift
+        lang_src lang_tgt true w st_src lc_src sc_src mem_src st_tgt lc_tgt sc_tgt mem_tgt.
+  Proof.
+    pcofix CIH. i. inv LIFT. pfold. ii. splits; ss.
+    { admit. }
+    { admit. }
+    { ii. punfold SIM. inv SIM. exploit TERMINAL; eauto. i. ss. des.
+
+    econs.
+
+    punfold SIM.
+
+
+    rever
+
+    punfold SIM.
+
+
+      Local.init TimeMap.bot Memory.init st_tgt Local.init TimeMap.bot Memory.init (JConfiguration.init_views, initial_finalized).
+  Proof.
+
 
   Lemma sim_lift_gsim lang_src lang_tgt sim_terminal
         (st_src: lang_src.(Language.state)) (st_tgt: lang_tgt.(Language.state))
-        (SIM: @sim_seq_all _ _ sim_terminal st_src st_tgt)
+        (SIM: @simo_seq_all _ _ sim_terminal st_src st_tgt)
     :
-    @sim_thread_past
+    @sim_thread
       world world_messages_le sim_memory sim_timemap sim_local
       lang_src lang_tgt sim_terminal false world_bot st_src Local.init TimeMap.bot Memory.init st_tgt Local.init TimeMap.bot Memory.init (JConfiguration.init_views, initial_finalized).
   Proof.
+
+
   Admitted.
 End LIFT.
